Code and wp proof for comparing lazy list of digits

theories/examples/lazy_int.v
@@ -7,18 +7,18 @@ From self.prelude Require Import base.
 From self.examples Require Import sample_int.
 
 Section lazy_int.
-  
+
   Context (PRED_CHUNK_BITS: nat).
   Definition CHUNK_BITS := S (PRED_CHUNK_BITS).
   Definition MAX_CHUNK := Z.ones CHUNK_BITS.
-  
+
   Context (PRED_NUM_CHUNKS: nat).
   Definition NUM_CHUNKS := S (PRED_NUM_CHUNKS).
-  
+
   Definition get_chunk : val :=
     λ: "α" "chnk",
       match: !"chnk" with
-        | NONE => 
+        | NONE =>
             let: "z" := sample_int PRED_CHUNK_BITS "α" in
             let: "next" := ref NONE in
             let: "val" := ("z", "next") in
@@ -27,8 +27,28 @@ Section lazy_int.
       | SOME "val" => "val"
       end.
 
+  Definition cmpZ : val :=
+    λ: "z1" "z2",
+      if: "z1" < "z2" then #(-1)
+      else
+        if: "z2" < "z1" then #1
+        else #0.
+
+  Definition cmp_list : val :=
+    rec: "cmp_list" "n" "α1" "cl1" "α2" "cl2" :=
+      if: "n" = #0 then
+        #0
+      else
+        let: "c1n" := get_chunk "α1" "cl1" in
+        let: "c2n" := get_chunk "α2" "cl2" in
+        let: "res" := cmpZ (Fst "c1n") (Fst "c2n") in
+        if: "res" = #0 then
+          "cmp_list" ("n" - #1) "α1" (Snd "c1n") "α2" (Snd "c2n")
+        else
+          "res".
+
   Context `{!prelogrelGS Σ}.
-  
+
   Fixpoint chunk_list l (zs : list Z) : iProp Σ :=
     match zs with
     | [] => l ↦ NONEV
@@ -80,5 +100,78 @@ Section lazy_int.
       { iExists _, _. iFrame. eauto. }
       { iIntros "Htail". iApply (chunk_and_tape_list_cons_chunk with "[$] [$]"). }
   Qed.
-  
+
+  Definition comparison2z c : Z :=
+    match c with
+    | Eq => 0
+    | Lt => -1
+    | Gt => 1
+    end.
+
+
+  Lemma wp_cmpZ (z1 z2 : Z) E :
+    {{{ True }}}
+      cmpZ #z1 #z2 @ E
+    {{{ RET #(comparison2z (Z.compare z1 z2)); True%I }}}.
+  Proof.
+    iIntros (Φ) "_ HΦ".
+    rewrite /cmpZ.
+    destruct (Z.compare_spec z1 z2).
+    - wp_pures; case_bool_decide; try lia.
+      wp_pures; case_bool_decide; try lia.
+      wp_pures. iApply "HΦ"; eauto.
+    - wp_pures; case_bool_decide; try lia.
+      wp_pures. iApply "HΦ"; eauto.
+    - wp_pures; case_bool_decide; try lia.
+      wp_pures; case_bool_decide; try lia.
+      wp_pures. iApply "HΦ"; eauto.
+  Qed.
+
+  Lemma wp_cmp_list n α1 α2 l1 l2 zs1 zs2 E :
+    n = length zs1 →
+    n = length zs2 →
+    {{{ chunk_and_tape_list α1 l1 zs1 ∗ chunk_and_tape_list α2 l2 zs2 }}}
+      cmp_list #n #lbl:α1 #l1 #lbl:α2 #l2 @ E
+    {{{ (z : Z), RET #z;
+        ⌜ z = comparison2z (digit_list_cmp zs1 zs2) ⌝ ∗
+        chunk_and_tape_list α1 l1 zs1 ∗ chunk_and_tape_list α2 l2 zs2 }}}.
+  Proof.
+    rewrite /cmp_list.
+    iIntros (Hlen1 Hlen2 Φ) "(Hzs1&Hzs2) HΦ".
+    iInduction n as [| n] "IH" forall (zs1 zs2 Hlen1 Hlen2 l1 l2).
+    - destruct zs1; last by (simpl in Hlen1; inversion Hlen1).
+      destruct zs2; last by (simpl in Hlen2; inversion Hlen2).
+      wp_pures. iModIntro. iApply "HΦ". iFrame. simpl; eauto.
+    - destruct zs1 as [| z1 zs1]; first by (simpl in Hlen1; inversion Hlen1).
+      destruct zs2 as [| z2 zs2]; first by (simpl in Hlen2; inversion Hlen2).
+      wp_pures.
+      wp_apply (wp_get_chunk with "Hzs1").
+      iIntros (l1') "(Hzs1'&Hclo1)".
+      wp_pures.
+      wp_apply (wp_get_chunk with "Hzs2").
+      iIntros (l2') "(Hzs2'&Hclo2)".
+      wp_pures. wp_apply (wp_cmpZ with "[//]").
+      iIntros "_". wp_pures.
+      case_bool_decide as Hcase.
+      { assert (z1 ?= z2 = Eq)%Z as Hzcmp.
+        { destruct (z1 ?= z2)%Z; try simpl in Hcase; try inversion Hcase. auto. }
+        wp_pure. wp_pure. wp_pure. wp_pure.
+        replace (Z.of_nat (S n) - 1)%Z with (Z.of_nat n); last by lia.
+        wp_apply ("IH" $! zs1 zs2 with "[] [] Hzs1' Hzs2'").
+        { eauto. }
+        { eauto. }
+        iIntros (res) "(%Heq&Hzs1&Hzs2)".
+        iDestruct ("Hclo1" with "Hzs1") as "Hzs1".
+        iDestruct ("Hclo2" with "Hzs2") as "Hzs2".
+        iApply "HΦ". iFrame.
+        iPureIntro. simpl. rewrite Hzcmp. eauto. }
+      { wp_pures.
+        iDestruct ("Hclo1" with "Hzs1'") as "Hzs1".
+        iDestruct ("Hclo2" with "Hzs2'") as "Hzs2".
+        iModIntro. iApply "HΦ"; iFrame.
+        iPureIntro. simpl. destruct (z1 ?= z2)%Z; try eauto.
+        simpl in Hcase; congruence.
+      }
+  Qed.
+
 End lazy_int.
